New Substitution

Basics.v
@@ -3,14 +3,62 @@ Inductive q : Type :=
   | qlin : q  (* [Figure 1-3, lin] *)
   | qun : q.  (* [Figure 1-3, un] *)
 
+Definition q_eq ( x : q ) ( y : q ) : bool :=
+  match x, y with
+  | qun, qun => true
+  | qlin, qlin => true
+  | _, _ => false
+  end.
+
+Example q_eq_test : q_eq qun qlin = false.
+Proof. simpl. reflexivity. Qed.
+
 (* Boolean Literal : True & False [Figure 1-3, b] *)
 Inductive b : Type :=
   | btrue : b    (* [Figure 1-3, true] *)
   | bfalse : b.  (* [Figure 1-3, false] *)
 
+Definition b_eq ( x : b ) ( y : b ) : bool :=
+  match x, y with
+  | btrue, btrue => true
+  | bfalse, bfalse => true
+  | _, _ => false
+  end.
+
+Example b_eq_test : b_eq btrue bfalse = false.
+Proof. simpl. reflexivity. Qed.
+
 (* Names of the Variables, [See Figure 1-3, x] *)
 Inductive id : Type :=
   | Id : nat -> id.
+
+Fixpoint nat_eq ( m : nat ) ( n : nat ) : bool :=
+  match m, n with
+  | O, O => true
+  | S _, O => false
+  | O, S _ => false
+  | S m', S n' => nat_eq m' n'
+  end.
+
+Lemma nat_eq_to_eq : forall m n, nat_eq m n = true -> m = n.
+Proof.
+  intros m. induction m; induction n; intros H.
+  - reflexivity.
+  - compute in H. inversion H.
+  - compute in H. inversion H.
+  - simpl in H. apply IHm in H. rewrite -> H. reflexivity.
+Qed.
+
+Definition var_eq ( x : id ) ( y : id ) : bool :=
+  match x, y with
+  | Id m, Id n => nat_eq m n
+  end.
+
+Lemma var_eq_to_eq : forall x y, var_eq x y = true -> x = y.
+Proof.
+  intros. destruct x. destruct y. inversion H. apply nat_eq_to_eq in H1.
+  rewrite -> H1. reflexivity.
+Qed.
 
 (* Type and Pretype *)
 Reserved Notation "'qty'" (at level 10).  (* [Figure 1-3, P] *)
@@ -26,6 +74,16 @@ Notation "T ** T'" := (ty_pair T T') (at level 20, left associativity).
 
 Notation "T --> T'" := (ty_arrow T T') (at level 40, left associativity).
 
+Fixpoint ty_eq ( T1 : ty ) ( T2 : ty ) : bool :=
+  match T1, T2 with
+  | ty_bool q1, ty_bool q2 => q_eq q1 q2
+  | ty_pair TT1 TT2 Q, ty_pair TT'1 TT'2 Q' => 
+    andb (q_eq Q Q') (andb (ty_eq TT1 TT'1) (ty_eq TT2 TT'2))
+  | ty_arrow TT1 TT2 Q, ty_arrow TT'1 TT'2 Q' => 
+    andb (q_eq Q Q') (andb (ty_eq TT1 TT'1) (ty_eq TT2 TT'2))
+  | _, _ => false
+  end.
+
 (* Terms [Figure 1-3, t] *)
 Inductive tm : Type :=
   | tmvar : id -> tm                       (* [Figure 1-3, x] *)
@@ -36,25 +94,34 @@ Inductive tm : Type :=
   | tmabs : q -> id -> ty -> tm -> tm      (* [Figure 1-3, q λx:T.t] *)
   | tmapp : tm -> tm -> tm.                (* [Figure 1-3, t t] *)
 
+Fixpoint tm_eq ( t1 : tm ) ( t2 : tm ) : bool :=
+  match t1, t2 with
+  | tmvar x, tmvar y => var_eq x y
+  | tmbool q1 x, tmbool q2 y => andb (q_eq q1 q2) (b_eq x y)
+  | tmif t1 t2 t3, tmif t'1 t'2 t'3 =>
+    andb (tm_eq t1 t'1) (andb (tm_eq t2 t'2) (tm_eq t3 t'3))
+  | tmpair q1 t1 t2, tmpair q'1 t'1 t'2 =>
+    andb (q_eq q1 q'1) (andb (tm_eq t1 t'1) (tm_eq t2 t'2))
+  | tmsplit t1 x y t2, tmsplit t'1 x' y' t'2 =>
+    andb (andb (var_eq x x') (var_eq y y')) (andb (tm_eq t1 t'1) (tm_eq t2 t'2))
+  | tmabs Q x T t, tmabs Q' x' T' t' =>
+    andb (andb (q_eq Q Q') (ty_eq T T')) (andb (var_eq x x') (tm_eq t t'))
+  | tmapp t1 t2, tmapp t'1 t'2 => andb (tm_eq t1 t'1) (tm_eq t2 t'2)
+  | _, _ => false
+  end.
+
+Example tm_eq_test_1 : tm_eq (tmvar (Id 0)) (tmvar (Id 0)) = true.
+Proof. simpl. reflexivity. Qed.
+
+Example tm_eq_test_2 : forall x y g,
+  x = tmvar (Id 0) ->
+  y = tmvar (Id 0) ->
+  g = tmbool qun bfalse ->
+  tm_eq (tmif g x y) (tmif g y x) = true.
+Proof. intros. rewrite -> H. rewrite -> H0. rewrite -> H1. 
+  simpl. reflexivity. Qed.
+
 (* Term Variable Replacement *)
-Fixpoint nat_eq ( m : nat ) ( n : nat ) : bool :=
-  match m, n with
-  | O, O => true
-  | S _, O => false
-  | O, S _ => false
-  | S m', S n' => nat_eq m' n'
-  end.
-
-Definition var_eq ( x : id ) ( y : id ) : bool :=
-  match x, y with
-  | Id m, Id n => nat_eq m n
-  end.
-
-Lemma var_eq_to_eq : forall x y, var_eq x y = true -> x = y.
-Proof.
-  intros. admit.
-Qed.
-
 Definition rpv ( x' : id ) ( x : id ) ( y : id ) : id :=  (* [x->y]x' *)
   if var_eq x x' then y else x'.
 
@@ -68,6 +135,57 @@ Fixpoint rp ( t : tm ) ( x : id ) ( y : id ) : tm :=  (* [x->y]t *)
   | tmabs qi x' T t => tmabs qi (rpv x' x y) T (rp t x y)
   | tmapp t1 t2 => tmapp (rp t1 x y) (rp t2 x y)
   end.
+
+(* Term Replacement *)
+Definition tmp : id := Id 999.
+
+Fixpoint rpt ( t : tm ) ( x : tm ) ( y : tm ) : tm :=
+  if tm_eq t x then y else
+  match t with
+  | tmif t1 t2 t3 => tmif (rpt t1 x y) (rpt t2 x y) (rpt t3 x y)
+  | tmpair qi t1 t2 => tmpair qi (rpt t1 x y) (rpt t2 x y)
+  | tmsplit t1 x1 x2 t2 => tmsplit (rpt t1 x y) x1 x2 (rpt t2 x y)
+  | tmabs qi x' T t => tmabs qi x' T (rp (rpt t (rp x x' tmp) y) tmp x')
+  | tmapp t1 t2 => tmapp (rpt t1 x y) (rpt t2 x y)
+  | _ => t
+  end.
+
+Example rpt_test_1 : forall x y X Y f qi T,
+  x = Id 0 ->
+  X = tmvar x ->
+  y = Id 1 ->
+  Y = tmvar y ->
+  f = tmabs qi x T (tmvar x) ->
+  rpt f X Y = f.
+Proof.
+  intros x y X Y f qi T Hx HX Hy HY Hf.
+  rewrite -> Hf.
+  rewrite -> HX.
+  rewrite -> HY.
+  rewrite -> Hx.
+  rewrite -> Hy.
+  simpl. compute. reflexivity.
+Qed.
+
+Example rpt_test_2 : forall x y X Y f qi T,
+  x = Id 0 ->
+  X = tmvar x ->
+  y = Id 1 ->
+  Y = tmvar y ->
+  f = tmabs qi x T (tmabs qi y T (tmpair qi X Y)) ->
+  rpt f (tmpair qi X Y) (tmpair qi Y X) = f.
+Proof.
+  intros x y X Y f qi T Hx HX Hy HY Hf.
+  rewrite -> Hf.
+  rewrite -> HX.
+  rewrite -> HY.
+  rewrite -> Hx.
+  rewrite -> Hy.
+  simpl.
+  assert (H : andb (q_eq qi qi) false = false).
+  { destruct qi; simpl; reflexivity. }
+  rewrite -> H. simpl. compute. reflexivity.
+Qed.
 
 (* Values and PreValues *)
 Reserved Notation "'pv'" (at level 10).  (* [Figure 1-7, w] *)
